Generalized reduction to MLWE

proof/security/MLWE.ec
@@ -608,6 +608,320 @@ qed.
 
 end SMP_vs_ROM.
 
+(* More interestingly, if one can prove a form of public indifferentiability
+   from the RO that samples matrices, we can co back to MLWE. *)
+theory SMP_vs_ROM_infinite.
+
+import MLWE_ROM.
+
+clone import MLWE_SMP.
+
+module type Simulator_t(O : RO_H.POracle) = {
+   include RO_SMP.POracle
+}.
+
+module type Distinguisher_t(O : RO_SMP.POracle) = {
+   proc interact(sd : seed, t : vector) : unit
+   proc distinguish(tr b : bool, _A : matrix) : bool 
+}.
+
+module WIndfReal(D : Distinguisher_t, S : Sampler, O : RO_SMP.Oracle) = {
+   proc main(tr b : bool) : bool = {
+        var sd,t,_A,b';
+        O.init();
+        sd <$ dseed;
+        t <$ duni;
+        D(O).interact(sd, t);
+        _A <@ S(O).sample(sd);
+        b' <@ D(O).distinguish(tr, b ,_A);
+        return b';
+   }
+}.
+
+module WIndfIdeal(D : Distinguisher_t, Sim : Simulator_t, O : RO_H.Oracle) = {
+   proc main(tr b : bool) : bool = {
+        var sd,t,_A,b';
+        O.init();
+        sd <$ dseed;
+        t <$ duni;
+        D(Sim(O)).interact(sd, t);
+        _A <@ O.o(sd);
+        b' <@ D(Sim(O)).distinguish(tr, b,_A);
+        return b';
+   }
+}.
+
+module (BS(Adv : SAdv_T, Sim : Simulator_t) : ROAdv_T) (O : RO_H.POracle) = {
+   proc guess(sd : seed, t : vector,uv : vector * R) = {
+       var b;
+       Adv(Sim(O)).interact(sd,t);
+       b <@ Adv(Sim(O)).guess(uv);
+       return b;
+   }
+}.
+
+import MLWE_vs_MLWE_ROM.
+
+module O = RO_H.Lazy.LRO.
+module OS = RO_SMP.Lazy.LRO.
+
+module (D(A : SAdv_T) : Distinguisher_t) (O : RO_SMP.POracle) = {
+  var _sd : seed
+  var _t : vector
+  proc interact(sd : seed, t : vector) : unit = {
+    _sd <- sd;
+    _t <- t;
+    A(O).interact(sd, t);                 
+  }
+  proc distinguish(tr b : bool, _A : matrix) : bool = {
+    var s,e,u0,u1,e',v0,v1,b';        
+    s <$ dshort;                                             
+    e <$ dshort;                                              
+    u0 <- (if tr then trmx _A else _A) *^ s + e;            
+    u1 <$ duni;                                               
+    e' <$ dshort_R;                                          
+    v0 <- (_t `<*>` s) &+ e';                                    
+    v1 <$ duni_R;                                    
+    b' <@ A(O).guess(if b then (u1, v1) else (u0, v0));
+    return b';
+  }
+}.
+
+
+import RO_H.
+clone import LazyEager.
+
+module DLeftAux(A : SAdv_T, Sim : Simulator_t)  (O : RO_H.POracle) = {
+     proc run(tr : bool,b : bool) : bool = {
+        var sd,t,_A,s,e,u0,u1,e',v0,v1,b';     
+        sd <$ dseed;
+        s <$ dshort;
+        e <$ dshort;
+        _A <@ O.o(sd);
+        _A <- if tr then trmx _A else _A;
+        u0 <- _A *^ s + e;
+        u1 <$ duni;
+        t <$ duni;
+        e' <$ dshort_R;
+        v0 <- (t `<*>` s) &+ e';
+        v1 <$ duni_R;
+        b' <@ BS(A, Sim, O).guess(sd, t,if b then (u1, v1) else (u0, v0)); 
+        return b';
+     }
+}.
+
+module (DLeft(A : SAdv_T, Sim : Simulator_t) : Distinguisher)  (O : RO_H.POracle) = {
+     proc run(b : bool) : bool = {
+         var b';
+         b' <@ DLeftAux(A,Sim,O).run(false,b);
+         return b';
+     }
+}.
+
+module (DLeftT(A : SAdv_T, Sim : Simulator_t) : Distinguisher)  (O : POracle) = {
+     proc run(b : bool) : bool = {
+         var b';
+         b' <@ DLeftAux(A,Sim,O).run(true,b);
+         return b';
+     }
+}.
+
+module DRightAux(A : SAdv_T, Sim : Simulator_t)   (O : POracle) = {
+     proc run(tr : bool, b : bool) : bool = {
+        var sd,t,_A,s,e,u0,u1,e',v0,v1,b';
+        sd <$ dseed;
+        t <$ duni;
+        A(Sim(O)).interact(sd, t);
+        _A <@ O.o(sd);
+        s <$ dshort;
+        e <$ dshort;
+        u0 <- (if tr then trmx _A else _A) *^ s + e;
+        u1 <$ duni;
+        e' <$ dshort_R;
+        v0 <- (t `<*>` s) &+ e';
+        v1 <$ duni_R;
+        b' <@ A(Sim(O)).guess(if b then (u1, v1) else (u0, v0));
+        return b';
+     }
+}.
+
+module (DRight(A : SAdv_T, Sim : Simulator_t) : Distinguisher)  (O : POracle) = {
+     proc run(b : bool) : bool = {
+         var b';
+         b' <@ DRightAux(A,Sim,O).run(false,b);
+         return b';
+     }
+}.
+
+module (DRightT(A : SAdv_T, Sim : Simulator_t) : Distinguisher)  (O : POracle) = {
+     proc run(b : bool) : bool = {
+         var b';
+         b' <@ DRightAux(A,Sim,O).run(true,b);
+         return b';
+     }
+}.
+
+
+lemma MLWE_SMP_equiv_lel tr b &m (A <: SAdv_T {-ERO, -RO_H.Lazy.LRO,-B,-Bt, -BS}) 
+                                 (Sim <: Simulator_t {-ERO, -RO_H.Lazy.LRO,-B,-Bt, -BS, -A}):
+  (forall (x : in_t), is_lossless (dout x)) =>
+  Pr[  MLWE_RO(BS(A,Sim),RO_H.Lazy.LRO).main(tr,b) @ &m : res] =
+  Pr[  MLWE_RO(BS(A,Sim),ERO).main(tr,b) @ &m : res].
+move => dout_ll.
+case (tr = false).
++ move => ->.
+  have left : forall &m0,
+           Pr[  MLWE_RO(BS(A,Sim),RO_H.Lazy.LRO).main(false, b) @ &m0 : res] = 
+           Pr[  Exp(RO_H.Lazy.LRO,DLeft(A,Sim)).main(b) @ &m0 : res].
+  + move => &m0; byequiv => //; last by smt().  
+    by proc; inline {2} 2;  inline {2} 3; sim; wp; conseq />;  sim.
+  have right : forall &m1, Pr[  MLWE_RO(BS(A,Sim),ERO).main(false,b) @ &m1 : res] = 
+                         Pr[  Exp(ERO,DLeft(A,Sim)).main(b) @ &m1 : res].
+  + move => &m0; byequiv => //; last by smt().  
+    by proc; inline {2} 2; inline {2} 3; sim; wp; conseq />;  sim.
+  have le : 
+     equiv [ Exp(RO_H.Lazy.LRO, DLeft(A,Sim)).main ~ Exp(ERO, DLeft(A,Sim)).main : 
+       ={glob DLeft(A,Sim),arg} ==> ={res}] by apply (eq_eager_sampling (DLeft(A,Sim)) dout_ll).
+  have ? : forall &m0 &m1 ,
+     (glob DLeft(A,Sim)){m0} = (glob DLeft(A,Sim)){m1} =>
+       Pr[Exp(RO_H.Lazy.LRO, DLeft(A, Sim)).main(b) @ &m0 : res] =
+       Pr[Exp(ERO, DLeft(A,Sim)).main(b) @ &m1 : res] 
+   by move => &m0 &m1 eqB; byequiv (le); smt().
+  by smt().
+move => *; have -> : tr by smt().
+have left : forall &m0,
+         Pr[  MLWE_RO(BS(A,Sim),RO_H.Lazy.LRO).main(true, b) @ &m0 : res] = 
+         Pr[  Exp(RO_H.Lazy.LRO,DLeftT(A,Sim)).main(b) @ &m0 : res].
++ move => &m0; byequiv => //; last by smt().  
+  by proc; inline {2} 2;  inline {2} 3; sim; wp; conseq />;  sim.
+have right : forall &m1, Pr[  MLWE_RO(BS(A,Sim),ERO).main(true,b) @ &m1 : res] = 
+                         Pr[  Exp(ERO,DLeftT(A,Sim)).main(b) @ &m1 : res].
++ move => &m0; byequiv => //; last by smt().  
+  by proc; inline {2} 2; inline {2} 3; sim; wp; conseq />;  sim.
+have le : 
+   equiv [ Exp(RO_H.Lazy.LRO, DLeftT(A,Sim)).main ~ Exp(ERO, DLeftT(A,Sim)).main : 
+       ={glob DLeftT(A,Sim),arg} ==> ={res}] by apply (eq_eager_sampling (DLeftT(A,Sim)) dout_ll).
+have ? : forall &m0 &m1 ,
+     (glob DLeft(A,Sim)){m0} = (glob DLeft(A,Sim)){m1} =>
+       Pr[Exp(RO_H.Lazy.LRO, DLeftT(A,Sim)).main(b) @ &m0 : res] =
+       Pr[Exp(ERO, DLeftT(A,Sim)).main(b) @ &m1 : res] 
+ by move => &m0 &m1 eqB; byequiv (le); smt().
+by smt().
+qed.
+
+lemma MLWE_SMP_equiv_ler tr b &m (A <: SAdv_T {-ERO,-RO_H.Lazy.LRO,-B,-Bt, -BS, -D})
+                                 (Sim <: Simulator_t {-A,-ERO,-RO_H.Lazy.LRO,-B,-Bt, -BS, -D}):
+  (forall (x : in_t), is_lossless (dout x)) =>
+  Pr[WIndfIdeal(D(A), Sim, O).main(tr, b) @ &m : res]=
+  Pr[WIndfIdeal(D(A), Sim, ERO).main(tr, b) @ &m : res].
+move => dout_ll.
+case (tr = false).
+move => ->.
++ have left : forall &m0,  
+          Pr[WIndfIdeal(D(A), Sim, O).main(false, b) @ &m0 : res] = 
+          Pr[ Exp(RO_H.Lazy.LRO,DRight(A,Sim)).main(b) @ &m0 : res].
+  + move => &m0; byequiv => //=; last by smt().
+    by proc; inline *; sim; auto => />. 
+  have right : forall &m1,
+             Pr[ WIndfIdeal(D(A), Sim, ERO).main(false, b) @ &m1 : res] = 
+             Pr[ Exp(ERO,DRight(A,Sim)).main(b) @ &m1 : res].
+  + move => &m1; byequiv => //=; last by smt().
+    by proc; inline *; sim; auto => />; sim.
+  have le : 
+     equiv [ Exp(RO_H.Lazy.LRO, DRight(A,Sim)).main ~ Exp(ERO, DRight(A,Sim)).main : 
+     ={glob DRight(A,Sim),arg} ==> ={res}] by apply (eq_eager_sampling (DRight(A,Sim)) dout_ll).
+  have ? : forall &m0 &m1 ,
+     (glob DLeft(A,Sim)){m0} = (glob DLeft(A,Sim)){m1} =>
+       Pr[Exp(RO_H.Lazy.LRO, DRight(A,Sim)).main(b) @ &m0 : res] =
+       Pr[Exp(ERO, DRight(A,Sim)).main(b) @ &m1 : res] 
+     by move => &m0 &m1 eqB; byequiv (le); smt().
+  by smt().
+move => *; have -> : tr by smt().
+have left : forall &m0,  
+      Pr[WIndfIdeal(D(A), Sim, O).main(true, b) @ &m0 : res] = 
+      Pr[ Exp(RO_H.Lazy.LRO,DRightT(A,Sim)).main(b) @ &m0 : res].
+  + move => &m0; byequiv => //=; last by smt().
+    by proc; inline *; sim; auto => />. 
+  have right : forall &m1,
+             Pr[ WIndfIdeal(D(A), Sim, ERO).main(true, b) @ &m1 : res] = 
+             Pr[ Exp(ERO,DRightT(A,Sim)).main(b) @ &m1 : res].
+  + move => &m1; byequiv => //=; last by smt().
+    by proc; inline *; sim; auto => />; sim.
+  have le : 
+     equiv [ Exp(RO_H.Lazy.LRO, DRightT(A,Sim)).main ~ Exp(ERO, DRightT(A,Sim)).main : 
+     ={glob DRightT(A,Sim),arg} ==> ={res}] by apply (eq_eager_sampling (DRightT(A,Sim)) dout_ll).
+  have ? : forall &m0 &m1 ,
+     (glob DLeftT(A,Sim)){m0} = (glob DLeftT(A,Sim)){m1} =>
+       Pr[Exp(RO_H.Lazy.LRO, DRightT(A,Sim)).main(b) @ &m0 : res] =
+       Pr[Exp(ERO, DRightT(A,Sim)).main(b) @ &m1 : res] 
+     by move => &m0 &m1 eqB; byequiv (le); smt().
+  by smt().
+qed.
+
+lemma MLWE_SMP_equiv b &m  (S <: Sampler {-O, -OS, -D}) 
+       (A <: SAdv_T {-ERO,-O, -OS, -B, -S, -D}) 
+       (Sim <: Simulator_t {-ERO, -O, -OS,-B,-Bt, -BS, -A, -D}):
+  (forall (x : in_t), is_lossless (dout x)) =>
+     Pr[ WIndfReal(D(A),S,OS).main(false,b) @ &m : res] = 
+     Pr[ WIndfIdeal(D(A),Sim,O).main(false,b) @ &m : res] =>
+  Pr[  MLWE(B(BS(A,Sim),O)).main(b) @ &m : res] =
+  Pr[  MLWE_SMP(A,S,OS).main(false,b) @ &m : res].
+proof.
+move => d_out_ll HSIM.
+rewrite -(MLWE_RO_equiv b &m (BS(A,Sim))).
+have -> : 
+    Pr[MLWE_SMP(A, S, OS).main(false, b) @ &m : res] = 
+    Pr[ WIndfReal(D(A),S,OS).main(false,b) @ &m : res]
+ by byequiv => //; proc; inline {2} 6; inline {2} 4; sim.
+rewrite HSIM.
+rewrite (MLWE_SMP_equiv_lel false b &m A Sim d_out_ll).
+rewrite (MLWE_SMP_equiv_ler false b &m A Sim d_out_ll).
+byequiv =>//;proc.  
+inline {1} 13; inline {2} 6; inline {2} 4.
+swap {1} [8..10] -3. swap{1} 12 -4. swap {1} 13 -10. swap {1} 14 -6. swap {1} 16 -4. 
+swap {2} 4 -1. swap {2} [13..14] -9. swap{2} 16 -10. swap{2} 17 -8. swap {2} 19 -9. 
+swap {1} 1 9. swap {2} 1 11. swap {2} 14 -1. 
+seq 9 9 : (!tr{2} /\  ={tr,b,glob A,glob Sim,sd,sd0,t0,s,e,u1,t,e',v1} /\ sd0{1} = sd{2} /\ t0{1} = t{2}); 
+   1: by inline *; auto.
+wp; call (_: ={glob ERO,glob Sim}); 1: by sim.
+wp;conseq (_: ={glob A, glob Sim, sd, sd0, t0,b,t} /\  sd0{1} = sd{2} /\ t0{1} = t{2} 
+          ==> ={glob A, glob Sim, ERO.m} /\ D._t{2} = t{1} /\ _A{1} = _A{2}); 1,2: smt().
+by inline *; sim; smt().
+qed.
+
+lemma MLWE_SMP_equiv_t b &m  (S <: Sampler {-O, -OS, -D}) 
+       (A <: SAdv_T {-ERO,-O, -OS, -B, -S, -D}) 
+       (Sim <: Simulator_t {-ERO, -O, -OS,-B,-Bt, -BS, -A, -D}):
+  (forall (x : in_t), is_lossless (dout x)) =>
+     Pr[ WIndfReal(D(A),S,OS).main(true,b) @ &m : res] = 
+     Pr[ WIndfIdeal(D(A),Sim,O).main(true,b) @ &m : res] =>
+  Pr[  MLWE(Bt(BS(A,Sim),O)).main(b) @ &m : res] =
+  Pr[  MLWE_SMP(A,S,OS).main(true,b) @ &m : res].
+proof.
+move => d_out_ll HSIM.
+rewrite -(MLWE_RO_equiv_t b &m (BS(A,Sim))).
+have -> : 
+    Pr[MLWE_SMP(A, S, OS).main(true, b) @ &m : res] = 
+    Pr[ WIndfReal(D(A),S,OS).main(true,b) @ &m : res]
+ by byequiv => //; proc; inline {2} 6; inline {2} 4; sim.
+rewrite HSIM.
+rewrite (MLWE_SMP_equiv_lel true b &m A Sim d_out_ll).
+rewrite (MLWE_SMP_equiv_ler true b &m A Sim d_out_ll).
+byequiv =>//;proc.  
+inline {1} 13; inline {2} 6; inline {2} 4.
+swap {1} [8..10] -3. swap{1} 12 -4. swap {1} 13 -10. swap {1} 14 -6. swap {1} 16 -4. 
+swap {2} 4 -1. swap {2} [13..14] -9. swap{2} 16 -10. swap{2} 17 -8. swap {2} 19 -9. 
+swap {1} 1 9. swap {2} 1 11. swap {2} 14 -1. 
+seq 9 9 : (tr{2} /\  ={tr,b,glob A,glob Sim,sd,sd0,t0,s,e,u1,t,e',v1} /\ sd0{1} = sd{2} /\ t0{1} = t{2}); 
+   1: by inline *; auto.
+wp; call (_: ={glob ERO,glob Sim}); 1: by sim.
+wp;conseq (_: ={glob A, glob Sim, sd, sd0, t0,b,t} /\  sd0{1} = sd{2} /\ t0{1} = t{2} 
+          ==> ={glob A, glob Sim, ERO.m} /\ D._t{2} = t{1} /\ _A{1} = _A{2}); 1,2: smt().
+by inline *; sim; smt().
+qed.
+
+end SMP_vs_ROM_infinite.
+
 (* FIXME_PY: THESE HINTS MAKE RND IMPOSSIBLY SLOW *)
 (* add duni_R_ll, duni_R_uni, duni_R_fu *)
 (* FIXME: without adding the hint explicitely the hint are lost after cloning *)
